Compile HO RILang to MLang

io/Compile.RILang.To.MLang.fst
@@ -5,128 +5,50 @@ open FStar.Tactics
 open FStar.Tactics.Typeclasses
 
 open Common
-
-open TC.Checkable
 open TC.Monitorable.Hist
 
-open IO.Sig
-open IIO
-
-open ILang
+open RILang
 open MLang
 
+let dm_mon (pi:monitorable_prop) : monad = {
+  m = rilang_dm pi;
+  ret = (fun (x:'a) -> IIO.dm_iio_return 'a x);
+  bind = (fun (m:rilang_dm pi 'a) (k:'a -> rilang_dm pi 'b) -> 
+    let wp : Hist.hist 'b = Hist.hist_bind (pi_as_hist #'a pi) (fun _ -> pi_as_hist pi) in 
+    let tr : IIO.dm_iio 'b wp = IIO.dm_iio_bind _ _ _ _ (as_iio_dm m) (fun x -> as_iio_dm (k x)) in
+    lemma_bind_pi_implies_pi #'a #'b pi;
+    let w = IIO.dm_iio_subcomp 'b wp (pi_as_hist pi) tr in
+    as_rilang_dm w)
+}
+
+assume val dm_acts (pi:monitorable_prop) : acts (dm_mon pi)
+
 class compilable (comp_in:Type u#a) (pi:monitorable_prop) = {
-  comp_out : Type u#a;
+  comp_out : Type u#b;
   compile: comp_in -> comp_out;
 
   [@@@no_method]
-  ilang_comp_in : ilang comp_in pi;
+  rilang_comp_in : rilang comp_in pi;
   [@@@no_method]
   mlang_comp_out : mlang comp_out;
 }
 
-class backtranslateable (btrans_out:Type u#a) (pi:monitorable_prop) = {
-  btrans_in : Type u#a;
-  backtranslate: btrans_in -> btrans_out;
-
-  [@@@no_method]
-  ilang_btrans_out : ilang btrans_out pi;
-  [@@@no_method]
-  mlang_btrans_in : mlang btrans_in;
-  [@@@no_method]
-  cc_pi:squash (forall h cmd arg. pi cmd arg h ==> io_pre cmd arg h);
-}
-
-class instrumentable (inst_in_in inst_in_out:Type) (pi:monitorable_prop) = {
-  inst_out_in : Type;
-  inst_out_out : Type;
-
-  instrument: (unverified_arrow inst_out_in inst_out_out pi) -> Tot (verified_arrow inst_in_in inst_in_out pi); 
-
-  [@@@no_method]
-  mlang_inst_in : mlang (unverified_arrow inst_out_in inst_out_out pi);
-  [@@@no_method]
-  ilang_inst_out : ilang (verified_arrow inst_in_in inst_in_out pi) pi;
-  [@@@no_method]
-  c_pi:squash (forall h cmd arg. pi cmd arg h ==> io_pre cmd arg h);
-}
-
-instance instrumentable_is_backtranslateable #t1 #t2 #pi (d1: instrumentable t1 t2 pi) : backtranslateable (verified_arrow t1 t2 pi) pi = {
-  btrans_in = unverified_arrow d1.inst_out_in d1.inst_out_out pi;
-  mlang_btrans_in = d1.mlang_inst_in;
-  backtranslate = d1.instrument;
-  ilang_btrans_out = d1.ilang_inst_out;
-  cc_pi = d1.c_pi;
-}
-
-(** *** Compilable base types **)
-
-instance compile_resexn pi (t:Type) {| d1:compilable t pi |} : compilable (resexn t) pi = {
-  ilang_comp_in = ilang_resexn pi t #d1.ilang_comp_in;
-
-  comp_out = resexn (d1.comp_out);
-  mlang_comp_out = mlang_resexn d1.comp_out #(d1.mlang_comp_out);
-
-  compile = (fun x ->
-    match x with
-    | Inl r -> Inl (compile r)
-    | Inr err -> Inr err)
-}
-
 (** *** Compilable arrows **)
-
-(** TODO: t1 and t2 are in universe 0. is that a problem? can we do HO? **)
-instance compile_verified_arrow
+instance compile_arrow
   pi
-  (t1:Type) {| d1:backtranslateable t1 pi |} 
+  (ct:((Type->Type)->Type)) {| d1:rilang (ct (dm_mon pi).m) pi |} {| d1':mlang (ct free.m) |}
   (t2:Type) {| d2:compilable t2 pi |} :
-  Tot (compilable (verified_arrow t1 t2 pi) pi) = {
-  ilang_comp_in = ilang_arrow pi t1 #d1.ilang_btrans_out t2 #d2.ilang_comp_in;
+  Tot (compilable ((ct (dm_mon pi).m) -> rilang_dm pi t2) pi) = {
+  rilang_comp_in = rilang_arrow pi d1 d2.rilang_comp_in;
 
-  comp_out = d1.btrans_in -> MIIO (resexn d2.comp_out);
-  mlang_comp_out = mlang_arrow d1.mlang_btrans_in d2.mlang_comp_out;
+  comp_out = (mon:monad -> acts mon -> ct mon.m) -> free.m d2.comp_out;
+  mlang_comp_out = mlang_free_arrow (mlang_effectpoly d1') d2.mlang_comp_out;
 
-  compile = (fun (f:verified_arrow t1 t2 pi) (x:d1.btrans_in) ->
-    let r : unit -> IIOpi _ pi = fun () -> Universe.raise_val (compile #_ #pi #(compile_resexn pi t2 #d2) (f (d1.backtranslate x))) in
-    let x : dm_iio _ _ = reify (r ()) in
-    let x' : dm_iio (Universe.raise_t (resexn d2.comp_out)) (fun p h -> forall r lt. b2t(enforced_locally pi h lt) ==> p lt r) = x in
-    assert (forall h. dm_iio_theta x' (fun lt r -> enforced_locally pi h lt) h);
-    let dm : dm_iio (resexn d2.comp_out) trivial_hist = Decorated (fun h lt -> b2t (enforced_locally pi h lt)) x' Return in
-    IIOwp?.reflect dm
+  compile = (fun (f:((ct (dm_mon pi).m) -> rilang_dm pi t2)) (tgt_x:(mon:monad -> acts mon -> ct mon.m)) ->
+    let src_x : ct (dm_mon pi).m = tgt_x (dm_mon pi) (dm_acts pi) in
+    let r : rilang_dm pi t2 = f src_x in
+    let r = as_iio_dm r in 
+    let w = IIO.dm_iio_bind _ _ _ (fun _ -> (pi_as_hist pi)) r (fun x -> IIO.dm_iio_return _ (d2.compile x)) in
+    w
   );
-}
-
-(** *** Backtranslate types **)
-instance backtranslateable_resexn pi (t:Type) {| d1:backtranslateable t pi |} : backtranslateable (resexn t) pi = {
-  ilang_btrans_out = ilang_resexn pi t #d1.ilang_btrans_out;
-
-  btrans_in = resexn (d1.btrans_in);
-  mlang_btrans_in = mlang_resexn d1.btrans_in #d1.mlang_btrans_in;
-
-  cc_pi = d1.cc_pi;
-  backtranslate = (fun x ->
-    match x with
-    | Inl r -> Inl (backtranslate r)
-    | Inr err -> Inr err)
-}
-
-(** *** Instrumentable arrows **)
-instance instrumentable_unverified_arrow 
-  pi
-  t1 {| d1:compilable t1 pi |}
-  t2 {| d2:backtranslateable t2 pi |} : 
-  instrumentable t1 t2 pi = {
-  mlang_inst_in = mlang_unverified_arrow pi d1.mlang_comp_out d2.mlang_btrans_in;
-
-  inst_out_in = d1.comp_out;
-  inst_out_out = d2.btrans_in;
-  ilang_inst_out = ilang_arrow pi t1 #d1.ilang_comp_in t2 #d2.ilang_btrans_out;
-
-  c_pi = d2.cc_pi;
-
-  instrument = (fun (f:unverified_arrow d1.comp_out d2.btrans_in pi) (x:t1) -> 
-    let (dm : (dm_iio (resexn d2.btrans_in) trivial_hist){ special_tree pi dm }) = reify (f (compile x)) in
-    let r  : resexn d2.btrans_in = MLang.InstrumentTo.ILang.instrument_mio dm pi #() #() #d2.cc_pi in 
-    backtranslate #_ #pi #(backtranslateable_resexn pi t2 #d2) r 
-  )
 }
